fstar/MLS.TreeSync.Symbolic.LeafNodeSignature.fst
@@ -55,7 +55,7 @@ let leaf_node_to_event #tkt ln_tbs =
 
 val leaf_node_has_event: #tkt:treekem_types dy_bytes -> principal -> timestamp -> leaf_node_tbs_nt dy_bytes tkt -> prop
 let leaf_node_has_event #tkt prin time ln_tbs =
-  did_event_occur_before time prin (leaf_node_to_event ln_tbs)
+  did_event_occur_before prin time (leaf_node_to_event ln_tbs)
 
 type group_has_tree_event (bytes:Type0) {|bytes_like bytes|} (tkt:treekem_types bytes) = {
   group_id: mls_bytes bytes;
@@ -99,7 +99,7 @@ let tree_to_event #tkt group_id (|l, i, t|) =
 
 val tree_has_event: #tkt:treekem_types dy_bytes -> principal -> timestamp -> mls_bytes dy_bytes -> (l:nat & i:tree_index l & treesync dy_bytes tkt l i) -> prop
 let tree_has_event #tkt prin time group_id (|l, i, t|) =
-  did_event_occur_before time prin (tree_to_event group_id (|l, i, t|))
+  did_event_occur_before prin time (tree_to_event group_id (|l, i, t|))
 
 val tree_has_equivalent_event: #l:nat -> #i:tree_index l -> tkt:treekem_types dy_bytes -> principal -> timestamp -> mls_bytes dy_bytes -> treesync dy_bytes tkt l i -> leaf_index l i -> prop
 let tree_has_equivalent_event #l #i tkt prin time group_id t li =
